\newcommand{\entree}{poids du bébé $P$}
\newcommand{\delentree}{du \entree}
\newcommand{\lentree}{le \entree}
\newcommand{\sortie}{couple moteur $C_m$}
\newcommand{\delasortie}{du \sortie}
\newcommand{\lasortie}{le \entree}
\newcommand{\correction}{
\begin{center}
 \includegraphics[width=0.2\linewidth]{img/schema_cin}
\end{center}

$\left\{T_{P\rightarrow 3}\right\}=\left\{\begin{array}{cc}
0 & 0 \\
-P & 0 \\
0 & 0
\end{array}\right\}_{C,R_0}$

$\left\{T_{C_m\rightarrow 1}\right\}=\left\{\begin{array}{cc}
0 & 0 \\
0 & 0 \\
0 & C_m
\end{array}\right\}_{A,R_0}$

$\left\{T_{0\rightarrow 1}\right\}=\left\{\begin{array}{cc}
X_{01} & L_{01} \\
Y_{01} & M_{01} \\
Z_{01} & 0
\end{array}\right\}_{A,R_0}$

$\left\{T_{1\rightarrow 2}\right\}=\left\{\begin{array}{cc}
X_{12} & L_{12} \\
Y_{12} & M_{12} \\
Z_{12} & 0
\end{array}\right\}_{B,R_0}=\left\{\begin{array}{cc}
X_{12} & L_{12}+l_1.sin\theta_1.Z_{12} \\
Y_{12} & M_{12}-l_1.cos\theta_1.Z_{12} \\
Z_{12} & l_1.(cos\theta_1.Y_{12}-sin\theta_1.X_{12})
\end{array}\right\}_{A,R_0}$

$\left\{T_{2\rightarrow 3}\right\}=\left\{\begin{array}{cc}
X_{23} & L_{23} \\
Y_{23} & M_{23} \\
Z_{23} & 0
\end{array}\right\}_{C,R_0}=\left\{\begin{array}{cc}
X_{23} & L_{23}+l(t).Z_{23} \\
Y_{23} & M_{23} \\
Z_{23} & -l(t).X_{23}
\end{array}\right\}_{A,R_0}$

$\left\{T_{0\rightarrow 3}\right\}=\left\{\begin{array}{cc}
X_{03} & L_{03} \\
0 & M_{03} \\
Z_{03} & N_{03}
\end{array}\right\}_{A,R_0}$

Isoler 1

$\left\{\begin{array}{l}
X_{01}-X_{12}=0 \\
Y_{01}-Y_{12}=0 \\
Z_{01}-Z_{12}=0 \\
L_{01}-L_{12}-l_1.sin\theta_1.Z_{12}=0 \\
M_{01}-M_{12}+l_1.cos\theta_1.Z_{12}=0 \\
-l_1.(cos\theta_1.Y_{12}-sin\theta_1.X_{12})+C_m=0
\end{array}\right.$

Isoler 2

$\left\{\begin{array}{l}
X_{12}-X_{23}=0 \\
Y_{12}-Y_{23}=0 \\
Z_{12}-Z_{23}=0 \\
L_{12}+l_1.sin\theta_1.Z_{12}-L_{23}-l(t).Z_{23}=0 \\
M_{12}-l_1.cos\theta_1.Z_{12}-M_{23}=0 \\
l_1.(cos\theta_1.Y_{12}-sin\theta_1.X_{12})+l(t).X_{23}=0
\end{array}\right.$

Isoler 3

$\left\{\begin{array}{l}
X_{23}+X_{03}=0 \\
Y_{23}-P=0 \\
Z_{23}+Z_{03}=0 \\
L_{23}+l(t).Z_{23}+L_{03}=0 \\
M_{23}+M_{03}=0 \\
N_{03}-l(t).X_{23}=0
\end{array}\right.$

~\ \\
$C_m=-l(t).X_{23}=-l(t).X_{12}$

$Y_{23}=P=Y_{12}$

$C_m=\frac{l_1.l(t).cos\theta_1}{l(t)-l_1.sin\theta_1}.P$
}

